case_study/RiscvPmp/Machine.v
@@ -168,7 +168,6 @@ Module Import RiscvPmpProgram <: Program RiscvPmpBase.
   | pmpWriteCfg           : Fun [cfg :: ty_pmpcfg_ent; value :: ty_byte] ty_pmpcfg_ent
   | pmpWriteAddr          : Fun [locked :: ty.bool; addr :: ty_xlenbits; value :: ty_xlenbits] ty_xlenbits
   | pmpCheck (bytes : nat) {H : restrict_bytes bytes} : Fun [addr ∷ ty_xlenbits; acc ∷ ty_access_type; priv ∷ ty_privilege] (ty.option ty_exception_type)
-  | pmpCheckExp (bytes : nat) {H : restrict_bytes bytes} : Fun [addr ∷ ty_xlenbits; acc ∷ ty_access_type; priv ∷ ty_privilege] (ty.option ty_exception_type)
   | pmpCheckPerms         : Fun [ent ∷ ty_pmpcfg_ent; acc ∷ ty_access_type; priv ∷ ty_privilege] ty.bool
   | pmpCheckRWX           : Fun [ent ∷ ty_pmpcfg_ent; acc ∷ ty_access_type] ty.bool
   | pmpMatchEntry         : Fun [addr ∷ ty_xlenbits; width :: ty_xlenbits; acc ∷ ty_access_type; priv ∷ ty_privilege; ent ∷ ty_pmpcfg_ent; pmpaddr ∷ ty_xlenbits; prev_pmpaddr ∷ ty_xlenbits] ty_pmpmatch
@@ -536,43 +535,6 @@ Module Import RiscvPmpProgram <: Program RiscvPmpBase.
     if: locked then addr else value.
 
   Definition fun_pmpCheck (bytes : nat) {H : restrict_bytes bytes} : Stm [addr ∷ ty_xlenbits; acc ∷ ty_access_type; priv ∷ ty_privilege] (ty.option ty_exception_type) :=
-    use lemma open_pmp_entries ;;
-    let: "width" :: ty_xlenbits := stm_call (to_bits xlen) [exp_val ty.int (Z.of_nat bytes)] in  
-    let: check%string :=
-      let: tmp1 := stm_read_register pmp0cfg in
-      let: tmp2 := stm_read_register pmpaddr0 in
-      let: tmp3 := exp_val ty_xlenbits [bv 0] in
-      let: tmp := call pmpMatchEntry addr width acc priv tmp1 tmp2 tmp3 in
-      match: tmp in pmpmatch with
-      | PMP_Success  => stm_val ty.bool true
-      | PMP_Fail     => stm_val ty.bool false
-      | PMP_Continue =>
-      let: tmp1 := stm_read_register pmp1cfg in
-      let: tmp2 := stm_read_register pmpaddr1 in
-      let: tmp3 := stm_read_register pmpaddr0 in
-      let: tmp := call pmpMatchEntry addr width acc priv tmp1 tmp2 tmp3 in
-      match: tmp in pmpmatch with
-      | PMP_Success  => stm_val ty.bool true
-      | PMP_Fail     => stm_val ty.bool false
-      | PMP_Continue =>
-          match: priv in privilege with
-          | Machine => stm_val ty.bool true
-          | User    => stm_val ty.bool false
-          end
-      end
-      end in
-      use lemma close_pmp_entries ;;
-      if: check
-      then None
-      else
-        match: acc in union access_type with
-        |> KRead pat_unit      => stm_exp (Some E_Load_Access_Fault)
-        |> KWrite pat_unit     => stm_exp (Some E_SAMO_Access_Fault)
-        |> KReadWrite pat_unit => stm_exp (Some E_SAMO_Access_Fault)
-        |> KExecute pat_unit   => stm_exp (Some E_Fetch_Access_Fault)
-        end.
-
-  Definition fun_pmpCheckExp (bytes : nat) {H : restrict_bytes bytes} : Stm [addr ∷ ty_xlenbits; acc ∷ ty_access_type; priv ∷ ty_privilege] (ty.option ty_exception_type) :=
     use lemma open_pmp_entries ;;
     let: "width" :: ty_xlenbits := stm_call (to_bits xlen) [exp_val ty.int (Z.of_nat bytes)] in  
     let: check%string :=
@@ -1199,7 +1161,6 @@ Module Import RiscvPmpProgram <: Program RiscvPmpBase.
     | pmpWriteCfg             => fun_pmpWriteCfg
     | pmpWriteAddr            => fun_pmpWriteAddr
     | @pmpCheck bytes H       => @fun_pmpCheck bytes H
-    | @pmpCheckExp bytes H    => @fun_pmpCheckExp bytes H
     | pmpCheckPerms           => fun_pmpCheckPerms
     | pmpCheckRWX             => fun_pmpCheckRWX
     | pmpMatchEntry           => fun_pmpMatchEntry
